**Name:** Stanley Goodwin
**Date:** 11/17/2024
**Collaborators:** None

---

$$\begin{align}
[\hat{x},\hat{y}]&=0
\end{align}$$
$$\begin{align}
[\hat{x},\hat{p}_y]&=x\cdot i\hbar\dfrac{\partial}{\partial y}- i\hbar\dfrac{\partial}{\partial y}x=0
\end{align}$$
$$\begin{align}
\bra{\psi}[\hat{y},\hat{p}_y]\ket{\psi}&=y\cdot i\hbar\dfrac{\partial}{\partial y}- i\hbar\dfrac{\partial}{\partial y}\cdot y
\end{align}$$
$$\begin{align}
...
\end{align}$$
$$\begin{align}
...
\end{align}$$
$$\begin{align}
...
\end{align}$$


### 2.1
Given $\Theta(\theta)=A\ln\left[\tan\left(\tfrac{\theta}{2}\right)\right]$, show it solves 
$$\begin{align}
\dfrac{\partial}{\partial\theta}\left(\sin\theta\dfrac{\partial}{\partial\theta}\Theta(\theta)\right)+\left[l(l+1)\sin^2\theta-m^2\right]\Theta(\theta)=0\\
\dfrac{\partial}{\partial\theta}\left(\sin\theta\dfrac{\partial}{\partial\theta}\Theta(\theta)\right)=0\\
\dfrac{\partial}{\partial\theta}\left(\sin\theta\dfrac{\partial}{\partial\theta}A\ln\left[\tan\left(\tfrac{\theta}{2}\right)\right]\right)=0\\
\end{align}$$




### 4.1
$$\begin{align}
V(r)&=\dfrac{1}{2m}\dfrac{l\hbar(l\hbar+\hbar)}{r^2}\approx\dfrac{(l\hbar)^2}{2mr^2}\\
&=\dfrac{(mvr)^2}{2mr^2}=\dfrac{m}{2}\dfrac{v^2}{r^2}r^2\\
&=\dfrac{(mvr)^2}{2mr^2}=\dfrac{m}{2}\omega^2r^2\\
&=\dfrac{4\pi^2mr^2}{2T^2}=2\pi^2\dfrac{MR^2}{T^2}\\
\Aboxed{V(r)&=2\pi^2\dfrac{MR^2}{T^2}}
\end{align}$$
Using Kepler's Laws $T^2=\dfrac{4\pi^2}{GM}r^3$, then:
$$\begin{align}
V(r)&=2\pi^2\dfrac{MR^2}{T^2}\\
V(r)&=\dfrac{1}{2}\dfrac{GM^2}{R}
\end{align}$$
